Prove that Backtracker.captureNext returns a correct capture group

correctness/RegexCorrectness/Backtracker/Path.lean
@@ -6,38 +6,44 @@ open Regex.Data (Span)
 
 namespace Regex.Backtracker
 
-inductive Path (nfa : NFA) (wf : nfa.WellFormed) : Span → Fin nfa.nodes.size → List (Nat × String.Pos) → Prop where
-  | init {l r} : Path nfa wf ⟨l, [], r⟩ ⟨nfa.start, wf.start_lt⟩ []
-  | more {i j : Fin nfa.nodes.size} {span₁ span₂ update₁ update₂ update₃} (prev : Path nfa wf span₁ i update₁) (step : nfa.Step 0 i span₁ j span₂ update₂)
+inductive Path (nfa : NFA) (wf : nfa.WellFormed) (l r : List Char) : Span → Fin nfa.nodes.size → List (Nat × String.Pos) → Prop where
+  | init : Path nfa wf l r ⟨l, [], r⟩ ⟨nfa.start, wf.start_lt⟩ []
+  | more {i j : Fin nfa.nodes.size} {span₁ span₂ update₁ update₂ update₃} (prev : Path nfa wf l r span₁ i update₁) (step : nfa.Step 0 i span₁ j span₂ update₂)
     (equpdate : update₃ = update₁ ++ List.ofOption update₂) :
-    Path nfa wf span₂ j update₃
+    Path nfa wf l r span₂ j update₃
 
 namespace Path
 
-theorem eq_or_nfaPath {nfa : NFA} {wf : nfa.WellFormed} {span i update} (path : Path nfa wf span i update) :
-  ∃ l r,
-    (span = ⟨l, [], r⟩ ∧ i.val = nfa.start ∧ update = []) ∨
-    nfa.Path 0 nfa.start ⟨l, [], r⟩ i span update := by
+theorem span_eq {nfa : NFA} {wf : nfa.WellFormed} {l r span i update} (path : Path nfa wf l r span i update) :
+  l = span.l ∧ r = span.m.reverse ++ span.r := by
   induction path with
-  | @init l r =>
-    exists l, r
-    simp
+  | init => simp
   | @more i j span₁ span₂ update₁ update₂ update₃ prev step equpdate ih =>
-    have ⟨l, r, h⟩ := ih
-    exists l, r
-    match h with
+    match step.span_eq_or_next with
+    | .inl eq => simp [eq, ih]
+    | .inr ⟨c, r', eqr, eq⟩ => simp_all
+
+theorem string_eq {nfa : NFA} {wf : nfa.WellFormed} {l r span i update} (path : Path nfa wf l r span i update) :
+  span.toString = ⟨l ++ r⟩ := by
+  simp [Span.toString, ←path.span_eq]
+
+theorem eq_or_nfaPath {nfa : NFA} {wf : nfa.WellFormed} {l r span i update} (path : Path nfa wf l r span i update) :
+  (span = ⟨l, [], r⟩ ∧ i.val = nfa.start ∧ update = []) ∨
+  nfa.Path 0 nfa.start ⟨l, [], r⟩ i span update := by
+  induction path with
+  | init => simp
+  | @more i j span₁ span₂ update₁ update₂ update₃ prev step equpdate ih =>
+    match ih with
     | .inl ⟨eqspan, eqi, equpdate'⟩ =>
       simp [equpdate, equpdate']
-      exact .inr (.last (eqspan ▸ eqi ▸ step))
+      refine .inr (.last (eqspan ▸ eqi ▸ step))
     | .inr path =>
       simp [equpdate]
-      exact .inr (path.trans (.last step))
+      refine .inr (path.trans (.last step))
 
-theorem nfaPath_of_ne {nfa : NFA} {wf : nfa.WellFormed} {span i update} (path : Path nfa wf span i update) (ne : i.val ≠ nfa.start) :
-  ∃ l r, nfa.Path 0 nfa.start ⟨l, [], r⟩ i span update := by
-  have ⟨l, r, h⟩ := eq_or_nfaPath path
-  simp [ne] at h
-  exact ⟨l, r, h⟩
+theorem nfaPath_of_ne {nfa : NFA} {wf : nfa.WellFormed} {l r span i update} (path : Path nfa wf l r span i update) (ne : i.val ≠ nfa.start) :
+  nfa.Path 0 nfa.start ⟨l, [], r⟩ i span update := by
+  simpa [ne] using eq_or_nfaPath path
 
 end Path
 
