correctness/RegexCorrectness/Backtracker/Traversal.lean
@@ -116,26 +116,39 @@ theorem mem_of_mem_top_stack {entry stack'} (hstack : entry :: stack' = stack) :
 
 end
 
+/-
+Here, we consider a minimal invariant enough to prove the "soundness" of the backtracker; a capture group found by the backtracker indeed corresponds to a match by the regex.
+Therefore, we are only concenred about that the states in the stack are reachable from the start node starting from a particular position.
+
+NOTE: if we want to show that the backtracker is complete (i.e., if the regex matches a string, then the backtracker will find a capture group), we need new invariants
+about the visited set so that we can reason about the case the backtracker returns `.none`.
+
+Current candidates are:
+
+1. Closure under transition: ∀ (state, pos) ∈ visited, nfa.Step 0 state pos state' pos' → (state', pos') ∈ visited ∨ ∃ entry ∈ stack, entry.state = state' ∧ entry.it.poss = pos'
+  * At the end of the traversal, we can use this invariant to show that the visited set is a reflexive-transitive closure of the step relation.
+2. Upper bound of the visited set: ∀ (state, pos) ∈ visited, (state, pos) ∈ visisted₀ ∨ ∃ span, Path nfa wf l r span state update
+  * We'll strengthen `UpperInv` to give an upper bound of the visited set.
+  * Combined with the closure property, we can show that the traversal adds just the states reachable from the starting node at a particular position.
+3. The visited set doesn't contain the `.done` state.
+  * This implies that if the traversal returns `.none`, then there is no match starting from the particular position.
+-/
 section
 
 variable {nfa wf startIdx maxIdx visited stack update' visited'}
 
-/-
-TODO: add property of the visited so that we can know that visited is bounded by reachable states from the start node starting from a particular position.
-TODO: should we expand Path to take the starting span?
--/
-structure UpperInv (wf : nfa.WellFormed) (stack : List (StackEntry HistoryStrategy nfa startIdx maxIdx)) where
-  reachable : ∀ entry ∈ stack, ∃ span, span.iterator = entry.it.it ∧ Path nfa wf span entry.state entry.update
+structure UpperInv (wf : nfa.WellFormed) (l r : List Char) (stack : List (StackEntry HistoryStrategy nfa startIdx maxIdx)) where
+  reachable : ∀ entry ∈ stack, ∃ span, span.iterator = entry.it.it ∧ Path nfa wf l r span entry.state entry.update
 
-theorem path_done_of_some (hres : captureNextAux HistoryStrategy nfa wf startIdx maxIdx visited stack = (.some update', visited'))
-  (inv : UpperInv wf stack) :
-  ∃ state span, nfa[state] = .done ∧ Path nfa wf span state update' := by
-  induction visited, stack using captureNextAux.induct' HistoryStrategy nfa wf startIdx maxIdx with
+theorem path_done_of_some {l r} (hres : captureNextAux HistoryStrategy nfa wf startIdx maxIdx visited stack = (.some update', visited'))
+  (inv : UpperInv wf l r stack) :
+  ∃ state span, nfa[state] = .done ∧ Path nfa wf l r span state update' := by
+  induction visited, stack using captureNextAux.induct' HistoryStrategy nfa wf startIdx with
   | base visited => simp [captureNextAux_base] at hres
   | visited visited update state it eq stack' mem ih =>
     simp [captureNextAux_visited mem] at hres
-    have inv' : UpperInv wf stack' := by
-      have reachable entry (mem : entry ∈ stack') : ∃ span, span.iterator = entry.it.it ∧ Path nfa wf span entry.state entry.update :=
+    have inv' : UpperInv wf l r stack' := by
+      have reachable entry (mem : entry ∈ stack') : ∃ span, span.iterator = entry.it.it ∧ Path nfa wf l r span entry.state entry.update :=
         inv.reachable entry (by simp [mem])
       exact ⟨reachable⟩
     exact ih hres inv'
@@ -146,8 +159,8 @@ theorem path_done_of_some (hres : captureNextAux HistoryStrategy nfa wf startIdx
   | fail visited update state it eq stack' mem hn => simp [captureNextAux_fail mem hn] at hres
   | epsilon visited update state it eq stack' mem visited' state' hn ih =>
     rw [captureNextAux_epsilon mem hn] at hres
-    have inv' : UpperInv wf (⟨update, state', it, eq⟩ :: stack') := by
-      have reachable entry (mem : entry ∈ ⟨update, state', it, eq⟩ :: stack') : ∃ span, span.iterator = entry.it.it ∧ Path nfa wf span entry.state entry.update := by
+    have inv' : UpperInv wf l r (⟨update, state', it, eq⟩ :: stack') := by
+      have reachable entry (mem : entry ∈ ⟨update, state', it, eq⟩ :: stack') : ∃ span, span.iterator = entry.it.it ∧ Path nfa wf l r span entry.state entry.update := by
         simp at mem
         cases mem with
         | inl eq' =>
@@ -161,8 +174,8 @@ theorem path_done_of_some (hres : captureNextAux HistoryStrategy nfa wf startIdx
   | split visited update state it eq stack' mem visited' state₁ state₂ hn ih =>
     rw [captureNextAux_split mem hn] at hres
     let stack'' := ⟨update, state₁, it, eq⟩ :: ⟨update, state₂, it, eq⟩ :: stack'
-    have inv' : UpperInv wf stack'' := by
-      have reachable entry (mem : entry ∈ stack'') : ∃ span, span.iterator = entry.it.it ∧ Path nfa wf span entry.state entry.update := by
+    have inv' : UpperInv wf l r stack'' := by
+      have reachable entry (mem : entry ∈ stack'') : ∃ span, span.iterator = entry.it.it ∧ Path nfa wf l r span entry.state entry.update := by
         simp [stack''] at mem
         match mem with
         | .inl eq₁ =>
@@ -180,8 +193,8 @@ theorem path_done_of_some (hres : captureNextAux HistoryStrategy nfa wf startIdx
     exact ih hres inv'
   | save visited update state it eq stack' mem visited' offset state' hn update' ih =>
     rw [captureNextAux_save mem hn] at hres
-    have inv' : UpperInv wf (⟨update', state', it, eq⟩ :: stack') := by
-      have reachable entry (mem : entry ∈ ⟨update', state', it, eq⟩ :: stack') : ∃ span, span.iterator = entry.it.it ∧ Path nfa wf span entry.state entry.update := by
+    have inv' : UpperInv wf l r (⟨update', state', it, eq⟩ :: stack') := by
+      have reachable entry (mem : entry ∈ ⟨update', state', it, eq⟩ :: stack') : ∃ span, span.iterator = entry.it.it ∧ Path nfa wf l r span entry.state entry.update := by
         simp at mem
         cases mem with
         | inl eq' =>
@@ -194,8 +207,8 @@ theorem path_done_of_some (hres : captureNextAux HistoryStrategy nfa wf startIdx
     exact ih hres inv'
   | anchor_pos visited update state it eq stack' mem visited' a state' hn ht ih =>
     rw [captureNextAux_anchor_pos mem hn ht] at hres
-    have inv' : UpperInv wf (⟨update, state', it, eq⟩ :: stack') := by
-      have reachable entry (mem : entry ∈ ⟨update, state', it, eq⟩ :: stack') : ∃ span, span.iterator = entry.it.it ∧ Path nfa wf span entry.state entry.update := by
+    have inv' : UpperInv wf l r (⟨update, state', it, eq⟩ :: stack') := by
+      have reachable entry (mem : entry ∈ ⟨update, state', it, eq⟩ :: stack') : ∃ span, span.iterator = entry.it.it ∧ Path nfa wf l r span entry.state entry.update := by
         simp at mem
         cases mem with
         | inl eq' =>
@@ -208,15 +221,15 @@ theorem path_done_of_some (hres : captureNextAux HistoryStrategy nfa wf startIdx
     exact ih hres inv'
   | anchor_neg visited update state it eq stack' mem visited' a state' hn ht ih =>
     rw [captureNextAux_anchor_neg mem hn ht] at hres
-    have inv' : UpperInv wf stack' := by
-      have reachable entry (mem : entry ∈ stack') : ∃ span, span.iterator = entry.it.it ∧ Path nfa wf span entry.state entry.update :=
+    have inv' : UpperInv wf l r stack' := by
+      have reachable entry (mem : entry ∈ stack') : ∃ span, span.iterator = entry.it.it ∧ Path nfa wf l r span entry.state entry.update :=
         inv.reachable entry (by simp [mem])
       exact ⟨reachable⟩
     exact ih hres inv'
   | char_pos visited update state it eq stack' mem visited' c state' hn hnext hc ih =>
     rw [captureNextAux_char_pos mem hn hnext hc] at hres
-    have inv' : UpperInv wf (⟨update, state', it.next hnext, eq⟩ :: stack') := by
-      have reachable entry (mem : entry ∈ ⟨update, state', it.next hnext, eq⟩ :: stack') : ∃ span, span.iterator = entry.it.it ∧ Path nfa wf span entry.state entry.update := by
+    have inv' : UpperInv wf l r (⟨update, state', it.next hnext, eq⟩ :: stack') := by
+      have reachable entry (mem : entry ∈ ⟨update, state', it.next hnext, eq⟩ :: stack') : ∃ span, span.iterator = entry.it.it ∧ Path nfa wf l r span entry.state entry.update := by
         simp at mem
         cases mem with
         | inl eq' =>
@@ -235,22 +248,22 @@ theorem path_done_of_some (hres : captureNextAux HistoryStrategy nfa wf startIdx
     exact ih hres inv'
   | char_neg visited update state it eq stack' mem visited' c state' hn hnext hc ih =>
     rw [captureNextAux_char_neg mem hn hnext hc] at hres
-    have inv' : UpperInv wf stack' := by
-      have reachable entry (mem : entry ∈ stack') : ∃ span, span.iterator = entry.it.it ∧ Path nfa wf span entry.state entry.update :=
+    have inv' : UpperInv wf l r stack' := by
+      have reachable entry (mem : entry ∈ stack') : ∃ span, span.iterator = entry.it.it ∧ Path nfa wf l r span entry.state entry.update :=
         inv.reachable entry (by simp [mem])
       exact ⟨reachable⟩
     exact ih hres inv'
   | char_end visited update state it eq stack' mem visited' c state' hn hnext ih =>
     rw [captureNextAux_char_end mem hn hnext] at hres
-    have inv' : UpperInv wf stack' := by
-      have reachable entry (mem : entry ∈ stack') : ∃ span, span.iterator = entry.it.it ∧ Path nfa wf span entry.state entry.update :=
+    have inv' : UpperInv wf l r stack' := by
+      have reachable entry (mem : entry ∈ stack') : ∃ span, span.iterator = entry.it.it ∧ Path nfa wf l r span entry.state entry.update :=
         inv.reachable entry (by simp [mem])
       exact ⟨reachable⟩
     exact ih hres inv'
   | sparse_pos visited update state it eq stack' mem visited' cs state' hn hnext hc ih =>
     rw [captureNextAux_sparse_pos mem hn hnext hc] at hres
-    have inv' : UpperInv wf (⟨update, state', it.next hnext, eq⟩ :: stack') := by
-      have reachable entry (mem : entry ∈ ⟨update, state', it.next hnext, eq⟩ :: stack') : ∃ span, span.iterator = entry.it.it ∧ Path nfa wf span entry.state entry.update := by
+    have inv' : UpperInv wf l r (⟨update, state', it.next hnext, eq⟩ :: stack') := by
+      have reachable entry (mem : entry ∈ ⟨update, state', it.next hnext, eq⟩ :: stack') : ∃ span, span.iterator = entry.it.it ∧ Path nfa wf l r span entry.state entry.update := by
         simp at mem
         cases mem with
         | inl eq' =>
@@ -269,15 +282,15 @@ theorem path_done_of_some (hres : captureNextAux HistoryStrategy nfa wf startIdx
     exact ih hres inv'
   | sparse_neg visited update state it eq stack' mem visited' cs state' hn hnext hc ih =>
     rw [captureNextAux_sparse_neg mem hn hnext hc] at hres
-    have inv' : UpperInv wf stack' := by
-      have reachable entry (mem : entry ∈ stack') : ∃ span, span.iterator = entry.it.it ∧ Path nfa wf span entry.state entry.update :=
+    have inv' : UpperInv wf l r stack' := by
+      have reachable entry (mem : entry ∈ stack') : ∃ span, span.iterator = entry.it.it ∧ Path nfa wf l r span entry.state entry.update :=
         inv.reachable entry (by simp [mem])
       exact ⟨reachable⟩
     exact ih hres inv'
   | sparse_end visited update state it eq stack' mem visited' cs state' hn hnext ih =>
     rw [captureNextAux_sparse_end mem hn hnext] at hres
-    have inv' : UpperInv wf stack' := by
-      have reachable entry (mem : entry ∈ stack') : ∃ span, span.iterator = entry.it.it ∧ Path nfa wf span entry.state entry.update :=
+    have inv' : UpperInv wf l r stack' := by
+      have reachable entry (mem : entry ∈ stack') : ∃ span, span.iterator = entry.it.it ∧ Path nfa wf l r span entry.state entry.update :=
         inv.reachable entry (by simp [mem])
       exact ⟨reachable⟩
     exact ih hres inv'
