correctness/RegexCorrectness/Data/BoundedIterator.lean
@@ -1,6 +1,8 @@
 import Regex.Data.BoundedIterator
 import RegexCorrectness.Data.String
 
+set_option autoImplicit false
+
 open String (Iterator)
 
 namespace Regex.Data.BoundedIterator
@@ -13,5 +15,24 @@ theorem next_valid {startIdx} (bit : BoundedIterator startIdx) (h : bit.hasNext)
   apply valid_of_it_valid
   simp [next, String.Iterator.next'_eq_next]
   exact (bit.valid_of_valid v).next h
+
+def ValidFor {startIdx} (l r : List Char) (bit : BoundedIterator startIdx) : Prop := bit.it.ValidFor l r
+
+namespace ValidFor
+
+theorem hasNext {startIdx l r} {bit : BoundedIterator startIdx} (vf : ValidFor l r bit) : bit.hasNext ↔ r ≠ [] := by
+  unfold ValidFor at vf
+  exact vf.hasNext
+
+theorem next {startIdx l c r} {bit : BoundedIterator startIdx} (vf : ValidFor l (c :: r) bit) : ValidFor (c :: l) r (bit.next (by simp [vf.hasNext])) := by
+  unfold ValidFor at vf
+  exact vf.next
+
+theorem next' {startIdx l r} {bit : BoundedIterator startIdx} (h : bit.hasNext) (vf : ValidFor l r bit) : ∃ c r', ValidFor (c :: l) r' (bit.next h) := by
+  match r with
+  | [] => simp [vf.hasNext] at h
+  | c :: r' => exact ⟨c, r', vf.next⟩
+
+end ValidFor
 
 end Regex.Data.BoundedIterator
