correctness/RegexCorrectness/Backtracker/Compile.lean
@@ -11,26 +11,29 @@ open Regex.Data (BoundedIterator Span)
 
 namespace Regex.Backtracker
 
-theorem captureNext.go.path_done_of_some {nfa wf startIdx bit} {update} {visited visited' : BitMatrix nfa.nodes.size (bit.maxIdx + 1 - startIdx)}
+theorem captureNext.go.path_done_of_some {nfa wf startIdx bit update} {visited visited' : BitMatrix nfa.nodes.size (bit.maxIdx + 1 - startIdx)}
   (v : bit.Valid) (hres : captureNext.go HistoryStrategy nfa wf startIdx bit visited = (.some update, visited')) :
-  ∃ state span, nfa[state] = .done ∧ Path nfa wf span state update := by
+  ∃ l r state span, span.toString = bit.it.toString ∧ nfa[state] = .done ∧ Path nfa wf l r span state update := by
   induction bit, visited using captureNext.go.induct' HistoryStrategy nfa wf startIdx with
   | found bit visited update' visited' haux =>
     simp [captureNext.go_found haux] at hres
     simp [hres] at haux
-    have inv₀ : captureNextAux.UpperInv wf [⟨[], ⟨nfa.start, wf.start_lt⟩, bit, rfl⟩] := by
+    have ⟨l, r, vf⟩ := (bit.valid_of_valid v).validFor
+    have inv₀ : captureNextAux.UpperInv wf l.reverse r [⟨[], ⟨nfa.start, wf.start_lt⟩, bit, rfl⟩] := by
       refine ⟨?_⟩
       simp
-      have ⟨l, r, vf⟩ := (bit.valid_of_valid v).validFor
-      exact ⟨⟨l.reverse, [], r⟩, (Span.validFor ⟨l.reverse, [], r⟩).eq_it (by simp [vf]), .init⟩
-    exact captureNextAux.path_done_of_some haux inv₀
+      have vfs := Span.validFor ⟨l.reverse, [], r⟩
+      simp at vfs
+      exact ⟨⟨l.reverse, [], r⟩, vfs.eq_it vf, .init⟩
+    have ⟨state, span, hn, path⟩ := captureNextAux.path_done_of_some haux inv₀
+    exact ⟨l.reverse, r, state, span, by simp [path.string_eq, vf.out], hn, path⟩
   | not_found_next bit visited visited' haux hnext ih =>
     simp [captureNext.go_not_found_next haux hnext] at hres
     exact ih (bit.next_valid hnext v) hres
   | not_found_end bit visited visited' haux hnext => simp [captureNext.go_not_found_end haux hnext] at hres
 
 theorem captureNext.path_done_of_some {nfa wf it update} (hres : captureNext HistoryStrategy nfa wf it = .some update) (v : it.Valid) :
-  ∃ state span, nfa[state] = .done ∧ Path nfa wf span state update := by
+  ∃ l r state span, span.toString = it.toString ∧ nfa[state] = .done ∧ Path nfa wf l r span state update := by
   if le : it.pos ≤ it.toString.endPos then
     simp [captureNext_le le] at hres
     let result := go HistoryStrategy nfa wf it.pos.byteIdx ⟨it, (Nat.le_refl _), le⟩ (BitMatrix.zero _ _)
@@ -45,11 +48,11 @@ theorem captureNext.capture_of_some_compile {e it update} (hres : captureNext Hi
     span.toString = it.toString ∧
     e.Captures ⟨l, [], r⟩ span groups ∧
     EquivUpdate groups update := by
-  have ⟨state, span, hn, path⟩ := captureNext.path_done_of_some hres v
+  have ⟨l, r, state, span, eqstring, hn, path⟩ := captureNext.path_done_of_some hres v
   have eq_zero := (NFA.done_iff_zero_compile rfl state).mp hn
   have ne : state.val ≠ (NFA.compile e).start := eq_zero ▸ Nat.ne_of_lt (NFA.lt_zero_start_compile rfl)
-  have ⟨l, r, path⟩ := path.nfaPath_of_ne ne
+  have path := path.nfaPath_of_ne ne
   have ⟨groups, eqv, c⟩ := NFA.captures_of_path_compile rfl (eq_zero ▸ path.compile_liftBound rfl)
-  exact ⟨l, r, span, groups, sorry, c, eqv⟩
+  exact ⟨l, r, span, groups, eqstring, c, eqv⟩
 
 end Regex.Backtracker
